killing an admit in Views.fst

src/arch/x64/Views.fst
@@ -79,10 +79,10 @@ let inverses32 (u:unit) : Lemma (inverses get32 put32) =
 let view32 = inverses32(); View 4 get32 put32
 
 let nat8s_to_nat64 (v1 v2 v3 v4 v5 v6 v7 v8:nat8) : nat64 =
-    v1 + 
-    v2 `op_Multiply` 0x100 + 
+    v1 +
+    v2 `op_Multiply` 0x100 +
     v3 `op_Multiply` 0x10000 +
-    v4 `op_Multiply` 0x1000000 + 
+    v4 `op_Multiply` 0x1000000 +
     v5 `op_Multiply` 0x100000000 +
     v6 `op_Multiply` 0x10000000000 +
     v7 `op_Multiply` 0x1000000000000 +
@@ -93,39 +93,60 @@ let get64_def (s:Seq.lseq UInt8.t 8) =
   nat8s_to_nat64
     (UInt8.v (Seq.index s 0))
     (UInt8.v (Seq.index s 1))
-    (UInt8.v (Seq.index s 2))    
+    (UInt8.v (Seq.index s 2))
     (UInt8.v (Seq.index s 3))
     (UInt8.v (Seq.index s 4))
     (UInt8.v (Seq.index s 5))
     (UInt8.v (Seq.index s 6))
-    (UInt8.v (Seq.index s 7))    
+    (UInt8.v (Seq.index s 7))
   )
 
+private
+abstract
+let get64_def_alt (s:Seq.lseq UInt8.t 8) : UInt64.t =
+  let open FStar.Mul in
+  let s0 = Seq.slice s 0 4 in
+  let u0 = get32_def s0 in
+  let s1 = Seq.slice s 4 8 in
+  let u1 = get32_def s1 in
+  UInt64.uint_to_t (UInt32.v u0 +
+                    UInt32.v u1 * 0x100000000)
+
+private
+let get64_def_alt_equiv (s:Seq.lseq UInt8.t 8)
+  : Lemma (get64_def s == get64_def_alt s)
+  = ()
+
 let put64_def (a:UInt64.t) : GTot (Seq.lseq UInt8.t 8) =
-  let s = Seq.create 8 (UInt8.uint_to_t 0) in
-  let x = UInt64.v a in
-  let s = Seq.upd s 0 (UInt8.uint_to_t (x % 0x100)) in
-  let x = x `op_Division` 0x100 in
-  let s = Seq.upd s 1 (UInt8.uint_to_t (x % 0x100)) in
-  let x = x `op_Division` 0x100 in
-  let s = Seq.upd s 2 (UInt8.uint_to_t (x % 0x100)) in
-  let x = x `op_Division` 0x100 in
-  let s = Seq.upd s 3 (UInt8.uint_to_t (x % 0x100)) in
-  let x = x `op_Division` 0x100 in
-  let s = Seq.upd s 4 (UInt8.uint_to_t (x % 0x100)) in
-  let x = x `op_Division` 0x100 in
-  let s = Seq.upd s 5 (UInt8.uint_to_t (x % 0x100)) in
-  let x = x `op_Division` 0x100 in
-  let s = Seq.upd s 6 (UInt8.uint_to_t (x % 0x100)) in
-  let x = x `op_Division` 0x100 in
-  let s = Seq.upd s 7 (UInt8.uint_to_t (x % 0x100)) in
-  s
+  let u0 = UInt32.uint_to_t (UInt64.v a % 0x100000000) in
+  let u1 = UInt32.uint_to_t ((UInt64.v a / 0x100000000) % 0x100000000) in
+  let s0 = put32_def u0 in
+  let s1 = put32_def u1 in
+  Seq.append s0 s1
+
+private
+let inverses64_def_aux (x:UInt64.t)
+  : Lemma (get64_def (put64_def x) == x)
+  = ()
+
+private
+let inverses64_def_aux' (x:Seq.lseq UInt8.t 8)
+  : Lemma (put64_def (get64_def x) `Seq.equal` x)
+  = reveal_opaque get32_def;
+    reveal_opaque put32_def;
+    inverses32();
+    get64_def_alt_equiv x;
+    get64_def_alt_equiv (put64_def (get64_def x));
+    inverses64_def_aux (get64_def x)
 
 let get64 = make_opaque get64_def
-let put64  = make_opaque put64_def
+let put64 = make_opaque put64_def
 
-//TODO
-let inverses64 (u:unit) : Lemma (inverses get64 put64) = admit()
+let inverses64 (u:unit) : Lemma (inverses get64 put64) =
+  reveal_opaque get64_def;
+  reveal_opaque put64_def;
+  Classical.forall_intro inverses64_def_aux;
+  Classical.forall_intro inverses64_def_aux'
 
 let view64 = inverses64 (); View 8 get64 put64
 
@@ -142,17 +163,17 @@ let get128_def (s:Seq.lseq UInt8.t 16) =
     (UInt8.v (Seq.index s 1))
     (UInt8.v (Seq.index s 2))    
     (UInt8.v (Seq.index s 3)))
- (nat8s_to_nat32
+  (nat8s_to_nat32
     (UInt8.v (Seq.index s 4))
     (UInt8.v (Seq.index s 5))
     (UInt8.v (Seq.index s 6))
     (UInt8.v (Seq.index s 7)))
- (nat8s_to_nat32
+  (nat8s_to_nat32
     (UInt8.v (Seq.index s 8))
     (UInt8.v (Seq.index s 9))
     (UInt8.v (Seq.index s 10))    
     (UInt8.v (Seq.index s 11)))
- (nat8s_to_nat32
+  (nat8s_to_nat32
     (UInt8.v (Seq.index s 12))
     (UInt8.v (Seq.index s 13))
     (UInt8.v (Seq.index s 14))
